Risc0/Gadgets/OneHot/Constraints/WeakestPresPart6.lean
@@ -16,39 +16,27 @@ def part₆_state (st: State) : State :=
             Option.get! (State.felts st { name := "output[2]" }))[felts][{ name := "outputSum-1" }] ←
         Option.get! (State.felts st { name := "output[0]+Output[1]" }) +
             Option.get! (State.felts st { name := "output[2]" }) -
-          Option.get!
-            ((st.felts[{ name := "outputSum" }] ←ₘ
-                Option.get! (State.felts st { name := "output[0]+Output[1]" }) +
-                  Option.get! (State.felts st { name := "output[2]" }))
-              { name := "1" }))[props][{ name := "andEqz outputSum-1" }] ←
+          Option.get! (State.felts st { name := "1" }))[props][{ name := "andEqz outputSum-1" }] ←
       ((Option.get! (State.props st { name := "andEqz output[1]<=1" }) ∧
           Option.get! (State.felts st { name := "output[2]<=1" }) = 0) ∧
         Option.get! (State.felts st { name := "output[0]+Output[1]" }) +
               Option.get! (State.felts st { name := "output[2]" }) -
-            Option.get!
-              ((st.felts[{ name := "outputSum" }] ←ₘ
-                  Option.get! (State.felts st { name := "output[0]+Output[1]" }) +
-                    Option.get! (State.felts st { name := "output[2]" }))
-                { name := "1" }) =
+            Option.get! (State.felts st { name := "1" }) =
           0))
-
--- Run the whole program by using part₆_state rather than Code.part₆
-def part₆_state_update (st: State): State :=
-  part₆_state st
 
 -- Prove that substituting part₆_state for Code.part₆ produces the same result
 lemma part₆_wp {st : State} :
   Code.getReturn (MLIR.runProgram Code.part₆ st) ↔
-  Code.getReturn (part₆_state_update st) := by
+  Code.getReturn (part₆_state st) := by
   unfold MLIR.runProgram; simp only
   unfold Code.part₆
   MLIR
-  unfold part₆_state_update part₆_state
+  unfold part₆_state
   rfl
 
 lemma part₆_updates_opaque {st : State} : 
   Code.getReturn (part₅_state_update st) ↔
-  Code.getReturn (part₆_state_update (part₅_state st)) := by
+  Code.getReturn (part₆_state (part₅_state st)) := by
   simp [part₅_state_update, part₆_wp]
 
 end Risc0.OneHot.Constraints.WP
